changement dans ring specification du sign, division
git-svn-id: svn+ssh://scm.gforge.inria.fr/svn/coq/trunk@9591 85f007b7-540e-0410-9357-904b9bb8a0f7

contrib/setoid_ring/InitialRing.v
@@ -13,11 +13,11 @@ Require Import BinNat.
 Require Import Setoid.
 Require Import Ring_theory.
 Require Import Ring_polynom.
+Require Import Ring_zdiv.
 
 Set Implicit Arguments.
 
 Import RingSyntax.
-
 
 (* An object to return when an expression is not recognized as a constant *)
 Definition NotConstant := false.
@@ -100,12 +100,12 @@ Section ZMORPHISM.
   | _ => None
   end.
 
- Lemma get_signZ_th : sign_theory ropp req gen_phiZ get_signZ.
+ Lemma get_signZ_th : sign_theory Zopp Zeq_bool get_signZ.
  Proof.
   constructor.
   destruct c;intros;try discriminate.
   injection H;clear H;intros H1;subst c'.
-  simpl;rrefl.
+  simpl. unfold Zeq_bool. rewrite Zcompare_refl. trivial.
  Qed.
 
  
@@ -365,6 +365,72 @@ Section NMORPHISM.
 
 End NMORPHISM.
 
+
+Section GEN_DIV.
+  
+  Variables  (R : Type) (rO : R) (rI : R) (radd : R -> R -> R)
+              (rmul : R -> R -> R) (rsub : R -> R -> R) (ropp : R -> R)
+              (req : R -> R -> Prop) (C : Type) (cO : C) (cI : C)
+              (cadd : C -> C -> C) (cmul : C -> C -> C) (csub : C -> C -> C)
+              (copp : C -> C) (ceqb : C -> C -> bool) (phi : C -> R).
+ Variable Rsth : Setoid_Theory R req.
+ Variable Reqe : ring_eq_ext radd rmul ropp req.
+ Variable ARth : almost_ring_theory rO rI radd rmul rsub ropp req.
+ Variable morph : ring_morph rO rI radd rmul rsub ropp req cO cI cadd cmul csub copp ceqb phi.
+ 
+  (* Usefull tactics *)		  
+  Add Setoid R req Rsth as R_set1.
+ Ltac rrefl := gen_reflexivity Rsth.
+  Add Morphism radd : radd_ext.  exact (Radd_ext Reqe). Qed.
+  Add Morphism rmul : rmul_ext.  exact (Rmul_ext Reqe). Qed.
+  Add Morphism ropp : ropp_ext.  exact (Ropp_ext Reqe). Qed.
+  Add Morphism rsub : rsub_ext. exact (ARsub_ext Rsth Reqe ARth). Qed.
+ Ltac rsimpl := gen_srewrite 0 1 radd rmul rsub ropp req Rsth Reqe ARth.
+
+ Definition triv_div x y :=  
+   if ceqb x y then (cI, cO)
+   else (cO, x).
+
+ Ltac Esimpl :=repeat (progress (
+   match goal with
+   | |- context [phi cO] => rewrite (morph0 morph)
+   | |- context [phi cI] => rewrite (morph1 morph)
+   | |- context [phi (cadd ?x  ?y)] => rewrite ((morph_add morph) x y)
+   | |- context [phi (cmul ?x  ?y)] => rewrite ((morph_mul morph) x y)
+   | |- context [phi (csub ?x  ?y)] => rewrite ((morph_sub morph) x y)
+   | |- context [phi (copp ?x)] => rewrite ((morph_opp morph) x)
+   end)).
+
+ Lemma triv_div_th : Ring_theory.div_theory  req cadd cmul phi triv_div.
+ Proof.
+  constructor.
+  intros a b;unfold triv_div.
+  assert (X:= morph.(morph_eq) a b);destruct (ceqb a b).
+  Esimpl.
+  rewrite X; trivial.
+  rsimpl.
+  Esimpl;  rsimpl.
+Qed.
+
+ Variable zphi : Z -> R.
+
+ Lemma Ztriv_div_th : div_theory req Zplus Zmult zphi zdiv_eucl.
+ Proof.
+  constructor.
+  intros; generalize (zdiv_eucl_correct a b); case zdiv_eucl; intros; subst.
+  rewrite Zmult_comm; rsimpl.
+ Qed.
+
+ Variable nphi : N -> R.
+
+ Lemma Ntriv_div_th : div_theory req Nplus Nmult nphi ndiv_eucl.
+  constructor.
+  intros; generalize (ndiv_eucl_correct a b); case ndiv_eucl; intros; subst.
+  rewrite Nmult_comm; rsimpl.
+ Qed.
+
+End GEN_DIV.
+
  (* syntaxification of constants in an abstract ring:
     the inverse of gen_phiPOS 
     Why we do not reconnize only rI ?????? *)
@@ -461,31 +527,42 @@ Ltac gen_ring_pow set arth pspec :=
  | Some ?t => constr:(t)
  end.
 
-Ltac default_sign_spec morph :=
- match type of morph with
- | @ring_morph ?R ?r0 ?rI ?radd ?rmul ?rsub ?ropp ?req 
-               ?C ?c0 ?c1 ?cadd ?cmul ?csub ?copp ?ceq_b ?phi =>
-      constr:(mkhypo (@get_sign_None_th R ropp req C phi))
- | _ => fail 1 "ring anomaly : default_sign_spec" 
- end.
-
-Ltac gen_ring_sign set rspec morph sspec rk :=
- match sspec with
- | None =>
-   match rk with
-   | Abstract =>
-     match type of rspec with
-     | @ring_theory ?R ?rO ?rI ?radd ?rmul ?rsub ?ropp ?req =>
-       constr:(mkhypo (@get_signZ_th R rO rI radd rmul ropp req set))
-     | _ => default_sign_spec morph 
-     end
-   | _ => default_sign_spec morph 
-   end
+Ltac gen_ring_sign morph sspec :=
+  match sspec with
+  | None =>
+    match type of morph with
+    | @ring_morph ?R ?r0 ?rI ?radd ?rmul ?rsub ?ropp ?req  
+               Z ?c0 ?c1 ?cadd ?cmul ?csub ?copp ?ceqb ?phi =>
+       constr:(@mkhypo (sign_theory copp ceqb get_signZ) get_signZ_th)
+    | @ring_morph ?R ?r0 ?rI ?radd ?rmul ?rsub ?ropp ?req  
+               ?C  ?c0 ?c1 ?cadd ?cmul ?csub ?copp ?ceqb ?phi =>
+        constr:(mkhypo (@get_sign_None_th C copp ceqb))
+    | _ => fail 2 "ring anomaly : default_sign_spec"
+    end
  | Some ?t => constr:(t)
  end.
 
+Ltac default_div_spec set reqe arth morph :=
+ match type of morph with
+ | @ring_morph ?R ?r0 ?rI ?radd ?rmul ?rsub ?ropp ?req 
+               Z ?c0 ?c1 Zplus Zmult ?csub ?copp ?ceq_b ?phi =>
+      constr:(mkhypo (Ztriv_div_th set phi))
+ | @ring_morph ?R ?r0 ?rI ?radd ?rmul ?rsub ?ropp ?req 
+               N ?c0 ?c1 Nplus Nmult ?csub ?copp ?ceq_b ?phi =>
+      constr:(mkhypo (Ntriv_div_th set phi)) 
+ | @ring_morph ?R ?r0 ?rI ?radd ?rmul ?rsub ?ropp ?req 
+               ?C ?c0 ?c1 ?cadd ?cmul ?csub ?copp ?ceq_b ?phi =>
+      constr:(mkhypo (triv_div_th set reqe arth morph))
+ | _ => fail 1 "ring anomaly : default_sign_spec" 
+ end.
 
-Ltac ring_elements set ext rspec pspec sspec rk :=
+Ltac gen_ring_div set reqe arth morph dspec  :=
+ match dspec with
+ | None => default_div_spec set reqe arth morph   
+ | Some ?t => constr:(t)
+ end.
+ 
+Ltac ring_elements set ext rspec pspec sspec dspec rk :=
   let arth := coerce_to_almost_ring set ext rspec in
   let ext_r := coerce_to_ring_ext ext in
   let morph :=
@@ -502,41 +579,53 @@ Ltac ring_elements set ext rspec pspec sspec rk :=
        | ring_morph _ _ _ _ _ _ _  _ _ _ _ _ _  _ _ => m 
        | @semi_morph _ _ _ _ _ _  _ _ _ _ _  _ _   => 
            constr:(SRmorph_Rmorph set m) 
-       | _ => fail 2 " ici"
+       | _ => fail 2 "ring anomaly"
        end
     | _ => fail 1 "ill-formed ring kind"
     end in
   let p_spec := gen_ring_pow set arth pspec in
-  let s_spec := gen_ring_sign set rspec morph sspec rk in
-  fun f => f arth ext_r morph p_spec s_spec.
+  let s_spec := gen_ring_sign morph sspec in
+  let d_spec := gen_ring_div set ext_r arth morph dspec in
+  fun f => f arth ext_r morph p_spec s_spec d_spec.
 
 (* Given a ring structure and the kind of morphism,
    returns 2 lemmas (one for ring, and one for ring_simplify). *)
-Ltac ring_lemmas set ext rspec pspec sspec rk :=
+
+ Ltac ring_lemmas set ext rspec pspec sspec dspec rk :=
   let gen_lemma2 :=
     match pspec with
     | None => constr:(ring_rw_correct) 
     | Some _ => constr:(ring_rw_pow_correct)
     end in
-  ring_elements set ext rspec pspec sspec rk
-    ltac:(fun arth ext_r morph p_spec s_spec =>
-        match p_spec with
-        | mkhypo ?pp_spec =>
-        match s_spec with
-        | mkhypo ?ps_spec =>
-          let lemma1 := 
-            constr:(ring_correct set ext_r arth morph pp_spec) in
-          let lemma2 := 
-            constr:(gen_lemma2 _  _ _  _ _ _  _  _ set ext_r arth 
-                           _  _ _  _ _ _  _  _  _ morph 
-                           _ _ _ pp_spec
-                           _ ps_spec) in 
-          fun f => f arth ext_r morph lemma1 lemma2
-        | _ => fail 2 "bad sign specification"
-       end
-       | _ => fail 1 "bad power specification" 
+  ring_elements set ext rspec pspec sspec dspec rk
+    ltac:(fun arth ext_r morph p_spec s_spec d_spec =>
+       match type of morph with
+       | @ring_morph ?R ?r0 ?rI ?radd ?rmul ?rsub ?ropp ?req 
+               ?C ?c0 ?c1 ?cadd ?cmul ?csub ?copp ?ceq_b ?phi =>
+          let gen_lemma2_0 := 
+              constr:(gen_lemma2 R  r0 rI  radd rmul rsub ropp req set ext_r arth 
+                                C  c0 c1 cadd cmul csub copp ceq_b phi morph) in
+          match p_spec with
+          | @mkhypo (power_theory _ _ _ ?Cp_phi ?rpow) ?pp_spec =>      
+             let gen_lemma2_1 := constr:(gen_lemma2_0 _ Cp_phi rpow pp_spec) in
+             match d_spec with
+             | @mkhypo (div_theory _ _ _ _  ?cdiv) ?dd_spec =>
+                let gen_lemma2_2 := constr:(gen_lemma2_1 cdiv dd_spec) in
+                match s_spec with
+                | @mkhypo (sign_theory _ _ ?get_sign) ?ss_spec =>    
+                  let lemma2 := constr:(gen_lemma2_2 get_sign ss_spec) in 
+                  let lemma1 := 
+                    constr:(ring_correct set ext_r arth morph pp_spec dd_spec) in
+                  fun f => f arth ext_r morph lemma1 lemma2
+                | _ => fail 4 "ring: bad sign specification"
+                end
+             | _ => fail 3 "ring: bad coefficiant division specification"
+             end
+          | _ => fail 2 "ring: bad power specification"
+          end
+       | _ => fail 1 "ring internal error: ring_lemmas, please report"
        end).
- 
+
 (* Tactic for constant *)
 Ltac isnatcst t :=
   match t with
